FokkerChallenge.lean
@@ -42,3 +42,4 @@ import FokkerChallenge.TwoVarsAreNotEnough.U
 import FokkerChallenge.TwoVarsAreNotEnough.Final
 import FokkerChallenge.TwoVarsAreNotEnough.Subterms
 import FokkerChallenge.TwoVarsAreNotEnough.Nameable
+import FokkerChallenge.TwoVarsAreNotEnough.TwoVarBlocks
